compiler/proofs/pure_compilerProofScript.sml
@@ -19,7 +19,62 @@ val _ = set_grammar_ancestry
 
 val _ = new_theory "pure_compilerProof";
 
-(* ---- misc ---- *)
+Theorem compiler_correctness:
+  compile_to_ast c s = SOME cake ⇒
+    ∃pure_ce ns.
+      frontend c s = SOME (pure_ce, ns) ∧
+      safe_itree $ itree_of (exp_of pure_ce) ∧
+      itree_rel
+         (itree_of (exp_of pure_ce))
+         (itree_semantics cake)
+Proof
+  strip_tac \\ gvs [compile_to_ast_def,frontend_def,AllCaseEqs()]
+  \\ qabbrev_tac ‘e3 = transform_cexp c e1’
+  \\ qabbrev_tac ‘e2 = demands_analysis c e3’
+  \\ ‘letrecs_distinct (exp_of e3)’
+     by simp [Abbr ‘e3’, transform_cexp_letrecs_distinct]
+  \\ qspec_then ‘e3’ assume_tac demands_analysis_soundness \\ fs []
+  \\ gvs[DefnBase.one_line_ify NONE pure_inferenceTheory.to_option_def, AllCaseEqs()]
+  \\ drule_then strip_assume_tac infer_types_SOME
+  \\ gvs[pure_inferenceTheory.infer_types_def, pure_inferenceTheory.fail_def,
+         pure_typingTheory.namespace_init_ok_def, AllCaseEqs()] >>
+     drule $ INST_TYPE [alpha |-> ``:(mlstring,unit) map``] infer_top_level_typed >>
+     disch_then $ qspecl_then [`empty`,`e3`] assume_tac >> gvs[] >>
+     `cexp_wf e2 ∧ NestedCase_free e2 ∧
+      type_tcexp (append_ns initial_namespace ns') 0 [] [] (tcexp_of e2) (M Unit)` by (
+        gvs[pure_demands_analysisTheory.demands_analysis_def] >>
+        FULL_CASE_TAC >> gvs[] >>
+        qabbrev_tac `d = demands_analysis_fun Nil e3 (empty str_compare)` >>
+        PairCases_on `d` >> gvs[] >>
+        dxrule_then assume_tac $ cj 5 demands_analysis_fun_insert_seq >> gvs[] >>
+        dxrule_all_then assume_tac pure_typingPropsTheory.insert_seq_imps >> gvs[]) >>
+     dxrule well_typed_program_imps >> simp[] >>
+     impl_tac >- gvs[pure_tcexp_lemmasTheory.cexp_wf_tcexp_wf] >> strip_tac
+  \\ qsuff_tac ‘itree_of (exp_of e3) = itree_of (exp_of e2)’
+  >- (
+    disch_then $ rewrite_tac o single \\ simp[]
+    \\ irule_at Any pure_to_cakeProofTheory.pure_to_cake_correct
+    \\ fs [cns_ok_def, pure_typingTheory.namespace_init_ok_def, EXISTS_PROD]
+    )
+  \\ mp_tac safe_exp_app_bisim_F_IMP_same_itree
+  \\ gvs [pure_exp_relTheory.app_bisimilarity_eq]
+QED
+
+Theorem alternative_compiler_correctness:
+  frontend c s = SOME (pure_ce, ns)
+  ⇒ safe_itree $ itree_of (exp_of pure_ce) ∧
+    ∃cake.
+      compile_to_ast c s = SOME cake ∧
+      itree_rel
+         (itree_of (exp_of pure_ce))
+         (itree_semantics cake)
+Proof
+  strip_tac >> assume_tac $ Q.GEN `cake` compiler_correctness >>
+  gvs[compile_to_ast_alt_def]
+QED
+
+
+(********** AST <-> string **********)
 
 Definition string_to_ast_def:
   string_to_ast s =
@@ -42,9 +97,10 @@ Proof
   \\ fs [EVERY_MEM,MEM_MAP,PULL_EXISTS]
 QED
 
-(* ---- main theorem ---- *)
 
-Theorem pure_compiler_correct:
+(********** Correctness wrt strings **********)
+
+Theorem pure_compiler_to_string_correct:
   compile c s = SOME t ⇒
   ∃pure_ce ty cake_prog.
     string_to_cexp s = SOME (pure_ce,ty) ∧
